%%%%%%%%%%%%%%%%%%%%%%%%%%%%%%%%%%%%%%%%%%%%%%%%%%%%%%%%%%%%%%%%
%%%%%%%%%%%%%%%%%%%%%%%%%%%%%%%%%%%%%%%%%%%%%%%%%%%%%%%%%%%%%%%%
%%%%
%%%% This text file is part of the source of slides for
%%%% `Introduction to High-Performance Scientific Computing'
%%%% by Victor Eijkhout, copyright 2012
%%%%
%%%%%%%%%%%%%%%%%%%%%%%%%%%%%%%%%%%%%%%%%%%%%%%%%%%%%%%%%%%%%%%%
%%%%%%%%%%%%%%%%%%%%%%%%%%%%%%%%%%%%%%%%%%%%%%%%%%%%%%%%%%%%%%%%

\begin{figure}[tp]
  \begin{center}
    \leavevmode
    \vbox{
        \begin{tabbing}
          Compute $r^{(0)} = b - Ax^{(0)}$ for some initial guess $x^{(0)}$ \\
          {\bf for } \= $ i = 1, 2, \ldots$ \\
          \> {\bf solve} $Mz^{(i-1)}=r^{(i-1)}$\\
          \> $\rho_{i-1}=r^{(i-1)^T}z^{(i-1)}$\\
          \> {\bf if} \= $i = 1$ \\
          \> \> $p^{(1)} = z^{(0)}$ \\
          \> {\bf else} \\
          \> \>$\beta_{i-1} = \rho_{i-1} / \rho_{i-2} $ \\
          \> \>$p^{(i)} = z^{(i-1)} + \beta_{i-1}p^{(i-1)} $ \\
          \>{\bf endif} \\
          \> $q^{(i)}=Ap^{(i)}$ \\
          \>$\alpha_i = \rho_{i-1}/p^{(i)^T}q^{(i)}$ \\
          \>$x^{(i)} = x^{(i-1)} + \alpha_ip^{(i)} $ \\
          \>$r^{(i)} = r^{(i-1)} - \alpha_iq^{(i)} $ \\
          \>check convergence; continue if necessary \\
          {\bf end}
        \end{tabbing}
        }
  \end{center}
\end{figure}

% Local Variables: 
% mode: latex
% TeX-master: "report"
% End: 
